\chapter{Proof of Equation \ref{eq:differential_entropy_q}}\label{entropy_proof}

In this appendix we will prove equation \ref{eq:differential_entropy_q} parting from equation \ref{eq:differential_entropy} (see page \pageref{eq:differential_entropy}).

Les $X$ be a continuous random variable with cumulative distribution function $F(x)$. Then, its quantile function is defined as:
\begin{equation}
Q(p) = F^{-1}(p) = \inf\{x \in \mathbb{R} : p \leq F(x)\}
\end{equation}
for a probability $0 \leq p \leq 1$.

From the previous definition we obtain:
\begin{align} 
F(x) = F(Q(p)) = p \label{eq:quantile_cdf} \\ 
Q(p) = Q(F(x)) = x \label{eq:cdf_quant}
\end{align}

Applying the chain rule to equation \ref{eq:quantile_cdf}:
\begin{equation}\label{eq:cdf_identity}
\frac{dF(Q(p))}{dp} = \frac{dF(Q)}{dQ} \cdot \frac{dQ(p)}{dp} = f(Q(p)) \cdot Q'(p) = 1
\end{equation}

Now, take the differential entropy as defined in \ref{eq:differential_entropy} and, for simplicity, rewrite it as:
\begin{equation}
h(x) = - \int_{-\infty}^{+\infty} u(x) dx
\end{equation}

Applying the change of variables from \ref{eq:cdf_quant} we obtain the following integration limits:
\begin{align}
a = \lim_{x \to -\infty} F(x) = 0\\
b = \lim_{x \to +\infty} F(x) = 1
\end{align}

And the following integrand:
\begin{equation}
h(p) = - \int_{0}^{1} u(Q(p)) \cdot Q'(p) dp = - \int_{0}^{1} f(Q(p)) \cdot \ln(f(Q(p))) \cdot Q'(p) dp
\end{equation}
which, making use of equation \ref{eq:cdf_identity}, can be simplified to equation \ref{eq:differential_entropy_q}:
\begin{equation}
h(p) = -  \int_{0}^{1} \ln\left(f(Q(p))\right) dp = - \int_{0}^{1} \ln\left(\frac{1}{Q'(p)}\right) dp = \int_{0}^{1} \ln\left(Q'(p)\right) dp
\end{equation}